Machine/Machine.thy
@@ -20,4 +20,18 @@ where
     return r
    od"
 
+lemma tpm_lift_wp[wp]:
+  "\<forall>ss. \<lbrace>\<lambda>s. P (ss\<lparr> tpm := s \<rparr>)\<rbrace> m \<lbrace>\<lambda>r s'. Q r (ss\<lparr> tpm := s' \<rparr>)\<rbrace> \<Longrightarrow> \<lbrace>P\<rbrace> tpm_lift m \<lbrace>Q\<rbrace>"
+  unfolding tpm_lift_def apply wp unfolding valid_def
+proof -
+  fix s :: machine_state and r
+  let ?tpm_state = "tpm s"
+  assume a: "\<forall>ss s. P (ss\<lparr>tpm := s\<rparr>) \<longrightarrow> (\<forall>(r, s')\<in>fst (m s). Q r (ss\<lparr>tpm := s'\<rparr>))"
+     and "P s"
+  have s: "s = s\<lparr>tpm := ?tpm_state\<rparr>" by auto
+  with `P s` have "P (s\<lparr>tpm := ?tpm_state\<rparr>)" by presburger
+  with a have "\<forall>(r, s')\<in>fst (m ?tpm_state). Q r (s\<lparr>tpm := s'\<rparr>)" by simp
+  thus "\<forall>x\<in>fst (m (tpm s)). (case x of (r, tpm_state') \<Rightarrow> \<lambda>s. Q r (s\<lparr>tpm := tpm_state'\<rparr>)) s" by auto
+qed
+
 end
